theories/Spilling/SpillMaxKill.v
@@ -1,8 +1,9 @@
 Require Import List Map Env AllInRel Exp MoreList.
 Require Import IL Annotation.
-Require Import Liveness.Liveness.
+Require Import Liveness.Liveness RenamedApart.
 Require Import ExpVarsBounded SpillSound OneOrEmpty RegLive.
 Require Import Take TakeSet.
+
 
 
 Set Implicit Arguments.
@@ -32,13 +33,14 @@ Inductive spill_max_kill (k:nat) :
       (sl : spilling)
       (rlv : ann ⦃var⦄)
     : let K := (R \ (Exp.freeVars e ∪ getAnn rlv)) ∪ (R ∩ L) in
+      let Kx:= ((R \ K ∪ L) \ getAnn rlv) in 
       Sp ⊆ R
       -> L ⊆ Sp ∪ M
-      -> spill_max_kill k ZL Λ (getAnn rlv, Sp ∪ M) s rlv sl
+      -> spill_max_kill k ZL Λ ({x; (R\K ∪ L) \ Kx}, Sp ∪ M) s rlv sl
       -> Exp.freeVars e ⊆ R\K ∪ L
       -> k > 0
       -> cardinal (R\K ∪ L) <= k
-      -> cardinal (getAnn rlv) <= k
+      -> cardinal {x; (R\K ∪ L) \ Kx} <= k
       -> spill_max_kill k ZL Λ (R,M) (stmtLet x e s) (ann1 Rlv rlv) (ann1 (Sp,L,nil) sl)
                        
   | SpillReturn
@@ -46,11 +48,11 @@ Inductive spill_max_kill (k:nat) :
       (Λ : list (⦃var⦄ * ⦃var⦄))
       (R M Sp L Rlv: ⦃var⦄)
       (e : op)
-    : let K := set_take ((cardinal R + cardinal L) - k) (R \ Op.freeVars e) in 
+    : let K := (R \ (Op.freeVars e)) ∪ (R ∩ L) in
       Sp ⊆ R
       -> L ⊆ Sp ∪ M
       -> Op.freeVars e ⊆ R\K ∪ L
-      -> cardinal ((R\K) ∪ L) <= k
+      -> cardinal (R\K ∪ L) <= k
       -> spill_max_kill k ZL Λ (R,M) (stmtReturn e) (ann0 Rlv) (ann0 (Sp,L,nil))
 
   | SpillIf
@@ -61,13 +63,13 @@ Inductive spill_max_kill (k:nat) :
       (s t : stmt)
       (sl_s sl_t : spilling)
       (rlv1 rlv2 : ann ⦃var⦄)
-    : let K := set_take ((cardinal R + cardinal L) - k) ((R \ Op.freeVars e) \ (getAnn rlv1 ∪ getAnn rlv2)) in
+    : let K := (R \ (Op.freeVars e ∪ getAnn rlv1 ∪ getAnn rlv2)) ∪ (R ∩ L) in
       Sp ⊆ R
       -> L ⊆ Sp ∪ M
       -> Op.freeVars e ⊆ R\K ∪ L
       -> cardinal (R\K ∪ L) <= k
-      -> spill_max_kill k ZL Λ (R\K ∪ L, Sp ∪ M) s rlv1 sl_s
-      -> spill_max_kill k ZL Λ (R\K ∪ L, Sp ∪ M) t rlv2 sl_t
+      -> spill_max_kill k ZL Λ (R \ K ∪ L, Sp ∪ M) s rlv1 sl_s
+      -> spill_max_kill k ZL Λ (R \ K ∪ L, Sp ∪ M) t rlv2 sl_t
       -> spill_max_kill k ZL Λ (R,M) (stmtIf e s t) (ann2 Rlv rlv1 rlv2) (ann2 (Sp,L,nil) sl_s sl_t)
 
   | SpillApp
@@ -145,69 +147,129 @@ Proof.
   rewrite card. omega.
 Qed.
 
+Lemma incl_minus_union (X:Type) `{OrderedType X} (s t u : ⦃X⦄) :
+  t ⊆ u -> s \ t ∪ u [=] s ∪ u
+.
+Proof.
+  intros; cset_tac.
+Qed.
 
-Lemma spill_sound_spill_max_kill k ZL Λ R R' M G s sl rlv :
+Lemma rkl'_incl_rkl (X:Type) `{OrderedType X} (s s' t t1 t2 u v w : ⦃X⦄) (x : X) :
+  let t' := s' \ (t1 ∪ t2) ∪ (s' ∩ v) in
+  t1 ⊆ s \ t ∪ v
+  -> t2 ⊆ {x; (s \ t ∪ v) \ w}
+  -> s' ⊆ u
+  -> x ∉ u
+  -> s' \ t' ∪ v ⊆ s \ t ∪ v
+.
+Proof.
+  intros t' t1_incl t2_incl s'_incl x_nin.
+  subst t'.
+  cset_tac.
+(*  rewrite <-minus_union. rewrite incl_minus_union;[|clear;cset_tac].
+  rewrite minus_minus. rewrite t1_incl.
+  rewrite t2_incl. cset_tac.
+      cbn in R_sub; clear - R_sub H9. cset_tac.*)
+Qed.
+
+Lemma spill_sound_spill_max_kill k ZL Λ R R' M G s sl rlv ra :
   rlv === reg_live ZL (fst ⊝ Λ) G s sl
+  -> renamedApart s ra
   -> spill_sound k ZL Λ (R,M) s sl
   -> rlive_sound ZL (fst ⊝ Λ) s sl rlv
+  -> R' ∪ M ⊆ fst (getAnn ra)
   -> getAnn rlv ⊆ R'
   -> spill_max_kill k ZL Λ (R',M) s rlv sl
 .
 Proof.
-  intros rlv_eq spillSnd rlive rlv_sub'.
-  general induction spillSnd; invc rlive; invc rlv_eq; cbn in rlv_sub'.
-  - econstructor; eauto;
-      set (K' := set_take ((cardinal R' + cardinal L) - k)
-                          (R' \ ((Exp.freeVars e ∪ getAnn al) \ L)));
-      set (Kx':= set_take (1 + cardinal (R' \ K' ∪ L) - k) ((R' \ K' ∪ L) \ getAnn al)).
-    + rewrite H13. eauto.
-  (*  + eapply IHspillSnd; eauto.
-      assert (getAnn al ⊆ {x;(R0 \ K ∪ L) \ Kx}) by admit.
-      rewrite H5. eauto. 
-      enough (getAnn al \ singleton x ⊆ (R0 \ K ∪ L) \ Kx) as Hypo.
-      { rewrite <-Hypo. clear; cset_tac. }
-      rewrite <-inter_subset_equal with (s':=getAnn al);[| clear; cset_tac]. rewrite H17.
+  intros rlv_eq rena spillSnd rlive R_sub rlv_sub'.
+  general induction spillSnd; invc rlive; invc rlv_eq; invc rena; cbn in rlv_sub'.
+  - set (K' := R' \ (Exp.freeVars e ∪ getAnn al) ∪ (R' ∩ L)).
+    assert (R' \ K' ∪ L ⊆ R0 \ K ∪ L) as rkl'_in_rkl2.
+    {
+      clear - H1 H10 spillSnd R_sub H9.
+      eapply reg_live_R in spillSnd; [|eapply PIR2_refl; eauto]. cbn in spillSnd.
 
-      rewrite H5.
-      rewrite set_take_incl. rewrite minus_minus. setoid_rewrite <-incl_right at 3.
-      rewrite <-rlv_sub.
-      subst Kx'. rewrite set_take_incl. clear;cset_tac. *)
-    + rewrite <-minus_union.
-      assert (forall s t u : ⦃var⦄, t ⊆ u -> s \ t ∪ u [=] s ∪ u) as seteq
-          by (clear; intros; cset_tac).
-      rewrite seteq;[|clear;cset_tac].
+      apply ann_R_get in H10. rewrite reg_live_G_eq in H10.
+      eapply rkl'_incl_rkl; eauto.
+      - rewrite H10. apply union_incl_split; [eauto|clear;cset_tac].
+      - cbn in R_sub. clear - R_sub; cset_tac.
+    }
+    subst K'.
+    econstructor; eauto;
+      set (K' := R' \ (Exp.freeVars e ∪ getAnn al) ∪ (R' ∩ L)) in *;
+      set (Kx':= (R' \ K' ∪ L) \ getAnn al) in *.
+    + rewrite H13. eauto.
+    + eapply IHspillSnd; eauto.
+      * invc  H20. cbn. rewrite H14.
+        cbn in R_sub. apply union_incl_split.
+        -- apply add_struct_incl. rewrite !minus_incl. rewrite H0, H13, rlv_sub'.
+           clear - R_sub. cset_tac.
+        -- rewrite H13, rlv_sub', R_sub. clear; cset_tac.
+      * enough (getAnn al \ singleton x ⊆ (R' \ K' ∪ L) \ Kx') as Hypo.
+        { rewrite <-Hypo. clear; cset_tac. }
+        rewrite <-inter_subset_equal with (s':=getAnn al);[| clear; cset_tac]. rewrite H17.
+        subst K'. rewrite <-minus_union, minus_minus.
+        setoid_rewrite <-rlv_sub' at 1. apply not_incl_minus; [clear; cset_tac|].
+        subst Kx'. clear; cset_tac.
+    (*
+      setoid_rewrite <-union_subset_equal with (s0:=lv) at 8;[|eauto].
+      setoid_rewrite <-union_subset_equal with (s0:=M0) at 11;[|eauto].
+      setoid_rewrite <-H13 at 2. setoid_rewrite <-union_assoc at 2. setoid_rewrite union_assoc at 2.
+      setoid_rewrite <-H0 at 2.
+      rewrite H13. clear - H17. cset_tac.*)
+    + subst K'. rewrite <-minus_union. rewrite incl_minus_union;[|clear;cset_tac].
       rewrite minus_minus, <-rlv_sub'.
       apply Exp.freeVars_live in H16. clear - H16; cset_tac.
-    + rewrite <-minus_union.
-      assert (forall s t u : ⦃var⦄, t ⊆ u -> s \ t ∪ u [=] s ∪ u) as seteq
-          by (clear; intros; cset_tac).
-      rewrite seteq;[|clear;cset_tac].
+    + rewrite subset_cardinal with (s':=R0 \ K ∪ L); eauto.
+    + rewrite subset_cardinal with (s':={x; (R0 \ K ∪ L) \ Kx}); eauto.
       eapply reg_live_R in spillSnd; [|eapply PIR2_refl; eauto].
-      rewrite minus_minus. rewrite H1.
-      apply ann_R_get in H10. rewrite H10, reg_live_G_eq, spillSnd. cbn.
-      (* we need a guarantee that x ∉ R', then everything will be fine. *)
-      rewrite meet_comm, meet_in_left. admit. (*
-      rewrite <-rlv_sub'.
-      invc H10.
-      assert (getAnn al ⊆ (R0 \ K ∪ L)) by admit.
-      rewrite H5. clear - H3.
-      enough (R' ∩ (R0 \ K ∪ L ∪ (R0 \ K ∪ L)) ∪ L ⊆ R0 \ K ∪ L) as enaf by (rewrite enaf; eauto).
-      clear; cset_tac.
-      
-      apply card_RKL; eauto.
-      * clear; cset_tac.
-      * clear - H3. rewrite subset_cardinal;eauto.
-      * 
-      * subst K'. rewrite set_take_incl. clear;cset_tac.
-      * clear - H3. rewrite subset_cardinal; eauto.
-      * admit. (* card *)
-    + admit. (* card Kx *) *)
-    + eapply reg_live_R in spillSnd; [|eapply PIR2_refl; eauto].
-      apply ann_R_get in H10. rewrite H10, reg_live_G_eq, spillSnd. cbn.
-      clear - H4. rewrite union_comm, union_subset_equal; eauto. cset_tac.
+      subst Kx'. rewrite minus_minus.
+      rewrite rkl'_in_rkl2. apply incl_add_eq; split; [clear;cset_tac|].
+      rewrite H10, reg_live_G_eq, spillSnd. cbn. clear. cset_tac.
   - econstructor; eauto.
     + rewrite H8; eauto.
-    + 
-  
+    + rewrite <-minus_union.
+      rewrite incl_minus_union;[|clear;cset_tac].
+      rewrite minus_minus, <-rlv_sub'.
+      apply Op.freeVars_live in H10. clear - H10. cset_tac.
+    + rewrite <-minus_union. rewrite incl_minus_union;[|clear;cset_tac].
+      rewrite minus_minus. rewrite H1. rewrite subset_cardinal with (s':=R0 \ K ∪ L); eauto.
+      clear; cset_tac.
+  - eapply reg_live_R in spillSnd1 as spillSnd1'; [|eapply PIR2_refl; eauto].
+    eapply reg_live_R in spillSnd2 as spillSnd2'; [|eapply PIR2_refl; eauto].
+    (*apply ann_R_get in H10 as al1_eq. apply ann_R_get in H11 as al2_eq.*)
+    econstructor; eauto.
+    + rewrite H12; eauto.
+    + rewrite <-minus_union. rewrite incl_minus_union;[|clear;cset_tac].
+      rewrite minus_minus, <-rlv_sub'.
+      apply Op.freeVars_live in H16. clear - H16; cset_tac.
+    + rewrite <-minus_union. rewrite incl_minus_union;[|clear;cset_tac].
+      rewrite minus_minus. rewrite H1.
+      rewrite H10, reg_live_G_eq, spillSnd1'. cbn.
+      rewrite H11, reg_live_G_eq, spillSnd2'. cbn.
+      rewrite subset_cardinal with (s':=R0 \ K ∪ L); eauto. 
+      cbn in R_sub; clear - R_sub H9; cset_tac.
+    + eapply IHspillSnd1; eauto.
+      * invc  H21. cbn. rewrite H20. cbn in R_sub.
+        rewrite <-minus_union, minus_minus, H6, H17, H18, rlv_sub', H12.
+        setoid_rewrite H0 at 4. rewrite H12, rlv_sub'. clear - R_sub. cset_tac.
+      * rewrite <-inter_subset_equal with (s':=getAnn al1); [|clear;cset_tac]. setoid_rewrite H17 at 1.
+        rewrite <-minus_union, minus_minus. setoid_rewrite rlv_sub' at 1. clear; cset_tac.
+(*
+      setoid_rewrite <-union_subset_equal with (s0:=lv) at 7;[|eauto].
+      setoid_rewrite <-union_subset_equal with (s0:=M0) at 10;[|eauto].
+      setoid_rewrite <-H12 at 2. setoid_rewrite <-union_assoc at 2. setoid_rewrite union_assoc at 2.
+      setoid_rewrite <-H0 at 2.
+      rewrite H12. clear - H17. cset_tac.*)
+    + eapply IHspillSnd2; eauto.
       
+      * invc  H22. cbn. rewrite H20. cbn in R_sub.
+        rewrite <-minus_union, minus_minus, H6, H17, H18, rlv_sub', H12.
+        setoid_rewrite H0 at 4. rewrite H12, rlv_sub'. clear - R_sub. cset_tac.
+      * rewrite <-inter_subset_equal with (s':=getAnn al2); [|clear;cset_tac]. setoid_rewrite H18 at 1.
+        rewrite <-minus_union, minus_minus. setoid_rewrite rlv_sub' at 1. clear; cset_tac.
+  - admit.
+  - admit.
+Admitted.
 
