theories/Spilling/RepairSpillInv.v
@@ -1,21 +1,30 @@
-Require Import RepairSpill RegLive.
-Require Import SpillSound Annotation Liveness.Liveness.
-Require Import List Map IL Take TakeSet OneOrEmpty.
+Require Import RepairSpill RegLive SpillMaxKill.
+Require Import SpillSound Annotation Liveness.Liveness RenamedApart.
+Require Import List Map IL Take TakeSet OneOrEmpty AllInRel.
 
 Set Implicit Arguments.
 
 (** * Invariance on correct spillings *)
 
 (* assumptions missing *)
-Lemma repair_spill_inv k ZL Λ s lv sl R M G
-  : live_sound Imperative ZL (merge ⊝ Λ) s lv
+Lemma repair_spill_inv k ZL Λ s lv sl R M ra rlv
+  : (*let rlv := reg_live ZL (fst ⊝ Λ) G s sl in*)
+    renamedApart s ra
+    -> rlive_min k ZL Λ (R,M) s sl rlv
+    -> rlive_sound ZL (fst ⊝ Λ) s sl rlv
+    -> getAnn rlv ∪ M ⊆ fst (getAnn ra)
+    -> getAnn rlv ⊆ R
+    -> live_sound Imperative ZL (merge ⊝ Λ) s lv
     -> spill_sound k ZL Λ (R,M) s sl
-    -> sl === repair_spill k ZL Λ R M s lv (reg_live ZL (fst ⊝ Λ) G s sl) sl
+    -> sl === repair_spill k ZL Λ R M s rlv lv sl
 .
 Proof.
-  intros liveSnd spillSnd.
-  general induction sl; invc liveSnd; invc spillSnd; econstructor.
-  - assert (H10' := H10). assert (H9' := H9).
+  intros rena rliveMin rliveSnd rlv_ra sub_R liveSnd spillSnd. 
+  eapply spill_sound_spill_max_kill in spillSnd; eauto;
+    [|reflexivity].
+  clear rena rlv_ra.
+  general induction sl; invc liveSnd; invc spillSnd; invc rlive.
+  - admit. (* assert (H10' := H10). assert (H9' := H9).
     assert (set_take_prefer k (L ∩ (Sp ∩ R ∪ M))
                               ((fst (nth (counted l) Λ ({},{}))
                                     \ of_list (nth (counted l) ZL nil)) \ R) [=] L) as Leq.
@@ -25,9 +34,9 @@ Proof.
             rewrite H16; clear; cset_tac).*)
     }
     econstructor; econstructor; symmetry;
-      apply inter_subset_equal in H9; apply inter_subset_equal in H10.
+      apply inter_subset_equal in H9; apply inter_subset_equal in H10. 
     + rewrite Leq. rewrite H9. apply union_subset_equal.
-      erewrite !get_nth; eauto. unfold fst,snd. rewrite H17.
+      erewrite !gect_nth; eauto. unfold fst,snd. rewrite H17.
       apply union_incl_split; [|clear;cset_tac].
       rewrite H18, H19. rewrite H10' at 1.
       assert (K [=] set_take (cardinal (R ∪ L) - k) (R \ R_f)) as Keq by admit.
@@ -39,17 +48,40 @@ Proof.
       assert (K [=] set_take (cardinal (R ∪ L) - k) (R \ R_f)) as Keq by admit.
       rewrite <-Keq.
       rewrite H18. clear; cset_tac.
-    + econstructor; eauto.
-  - assert (H6' := H6).
-    econstructor; econstructor; apply inter_subset_equal in H6;
-      eauto.
-    assert ((L ∩ (Sp ∩ R ∪ M)) [=] L) as Leq.
+    + econstructor; eauto. *)
+  - assert (Sp ∩ R [=] Sp) as Speq by (apply inter_subset_equal; rewrite H7, H3, sub_R; eauto).
+    econstructor; econstructor; [econstructor|]; eauto.
+    assert ((L ∩ (Sp ∩ R ∪ M)) [=] L) as Leq
+        by (apply inter_subset_equal in H8; rewrite Speq, H8; eauto).
+    rewrite set_take_prefer_eq; rewrite Leq; eauto.
+    + clear - H10. rewrite subset_cardinal; eauto.
+    + rewrite H9, H3, sub_R. clear; cset_tac.
+  - assert (Rlv = getAnn rlv) as Rlv_eq.
+    { clear - H8. destruct rlv; isabsurd. rewrite <-H8. cbn. reflexivity. }
+    cbn in H13, H18, Kx, H16. rewrite <-Rlv_eq in *.
+    assert (Sp ∩ R [=] Sp) as Speq by (apply inter_subset_equal; rewrite H13, sub_R; eauto).
+    assert (L ∩ (Sp ∩ R ∪ M) [=] L) as Leq
+        by (apply inter_subset_equal in H14; rewrite Speq, H14; eauto).
+    assert (L [=] (set_take_prefer k (L ∩ (Sp ∩ R ∪ M)) (Exp.freeVars e \ R))) as Leq'.
     {
-      apply inter_subset_equal in H7. rewrite H6, H7. eauto.
+      rewrite set_take_prefer_eq; rewrite Leq; eauto.
+      * clear - H18. rewrite subset_cardinal; eauto.
+      * rewrite H16, sub_R. clear; cset_tac.
     }
-    rewrite set_take_prefer_eq; eauto.
-    + rewrite Leq. rewrite subset_cardinal; eauto.
-    + rewrite H8, Leq. clear; cset_tac.
+    econstructor; [econstructor|]; [econstructor| |]; eauto.
+    + rewrite union_comm. setoid_rewrite Speq at 1. rewrite union_comm.
+      symmetry. rewrite union_subset_equal; eauto.
+      rewrite !set_take_least_avoid_eq.
+      * rewrite <-Leq'. cbn. rewrite minus_union. rewrite union_subset_equal; [|clear;cset_tac].
+        rewrite minus_union. eapply Exp.freeVars_live in H23.
+        -- admit.
+        -- admit.
+      * admit.
+      * admit. 
+    + rewrite set_take_prefer_eq; rewrite Leq; eauto.
+      * clear - H18. rewrite subset_cardinal; eauto.
+      * rewrite H16, H8, sub_R. clear; cset_tac.
+    + 
   - assert (H12' := H12); assert (H13' := H13).
     assert (Sp ∩ R [=] Sp) as Speq'
         by (apply inter_subset_equal; eauto).
@@ -62,8 +94,12 @@ Proof.
       - rewrite subset_cardinal; [apply H17|]; eauto.
       - rewrite H15; clear; cset_tac.
     }
-    econstructor; econstructor; symmetry;
+    econstructor; [econstructor|]; eauto; [econstructor|]; eauto.
+    + exploit IHsl as IH'; eauto. 
+    + admit.
+    + econstructor; symmetry;
       apply inter_subset_equal in H12; apply inter_subset_equal in H13.
     + admit.
     + apply Leq.
+  - 
       
